Rework Interfaces

src/Interfaces.v
@@ -5,18 +5,12 @@ From Equations Require Import Equations.
 
 From Coq Require Import Arith List Lia Setoid Morphisms.
 Import ListNotations.
-From Clairvoyance Require Import Core Approx ApproxM List Misc BankersQueue Launchbury Cost.
+From Clairvoyance Require Import Core Approx ApproxM List Misc BankersQueue Cost.
 
 Set Primitive Projections.
 Set Implicit Arguments.
 Set Contextual Implicit.
 Set Maximal Implicit Insertion.
-
-Definition option_bind {A B} (o : option A) (k : A -> option B) : option B :=
-  match o with
-  | None => None
-  | Some a => k a
-  end.
 
 (* lookups xs [n; m; p] = [xs!!n; xs!!m; xs!!p], or None if out of bounds *)
 Fixpoint lookups {A} (xs : list A) (ns : list nat) : option (list A) :=
@@ -27,133 +21,121 @@ Fixpoint lookups {A} (xs : list A) (ns : list nat) : option (list A) :=
     option_map (cons x) (lookups xs ns))
   end.
 
-Module Pure.
+Class PureImpl (op value : Type) : Type :=
+  eval_op : op -> list value -> list value.
 
-Record Impl (op : Type) : Type :=
-  { value : Type
-  ; raw_eval_op : op -> list value -> list value
-  }.
+Definition event (op : Type) : Type := (op * list nat).
+Definition trace (op : Type) : Type := list (event op).
+Definition stack (value : Type) : Type := list value.
 
-Definition eval_op {op : Type} {j : Impl op} (o : op) (ns : list nat) (xs : list j.(value))
-  : list j.(value) :=
-  match lookups xs ns with
-  | None => xs  (* noop *)
-  | Some vs => xs ++ j.(raw_eval_op) o vs
+Section Pure.
+
+Context {op value : Type} {j : PureImpl op value}.
+
+Definition eval_event '((o, ns) : event op) (vs : stack value) : stack value :=
+  match lookups vs ns with
+  | None => vs  (* noop *)
+  | Some xs => vs ++ eval_op o xs
   end.
 
-Fixpoint eval_ops {op : Type} {j : Impl op} (os : list (op * list nat)) (xs : list j.(value))
-  : list j.(value) :=
-  match os with
+Fixpoint eval_trace (es : trace op) (xs : stack value) : stack value :=
+  match es with
   | [] => xs
-  | (o, ns) :: os => eval_ops os (eval_op o ns xs)
+  | e :: es => eval_trace es (eval_event e xs)
   end.
 
-Module Cost.
+End Pure.
 
-Record Impl (op : Type) : Type :=
-  { impl :> Pure.Impl op
-    (* The cost may depend on the input *)
-  ; raw_cost : op -> list impl.(value) -> nat
-  }.
+(* The cost may depend on the input *)
+Class CostSpec (op value : Type) : Type :=
+  cost_op : op -> list value -> nat.
 
-Definition cost {op : Type} {j : Impl op} (o : op) (ns : list nat) (vs : list j.(value)) : nat :=
+Section Cost.
+
+Context {op value : Type} {pure_impl : PureImpl op value} {cost_spec : CostSpec op value}.
+
+Definition cost_event '((o, ns) : event op) (vs : stack value) : nat :=
   match lookups vs ns with
   | None => 0
-  | Some xs => j.(raw_cost) o xs
+  | Some xs => cost_op o xs
   end.
 
-Fixpoint eval {op : Type} {j : Impl op} (os : list (op * list nat)) (xs : list j.(value))
-  : nat :=
-  match os with
+Fixpoint cost_trace (es : trace op) (vs : stack value) : nat :=
+  match es with
   | [] => 0
-  | (o, ns) :: os => cost o ns xs + eval os (eval_op o ns xs)
+  | e :: es => cost_event e vs + cost_trace es (eval_event e vs)
   end.
 
 End Cost.
 
-End Pure.
+Class CvImpl (op valueA : Type) : Type :=
+  exec_op : op -> list valueA -> M (list valueA).
 
-Coercion Pure.Cost.impl : Pure.Cost.Impl >-> Pure.Impl.
+Section Cv.
 
-Notation raw_cost_op := Pure.Cost.raw_cost.
-Notation cost_op := Pure.Cost.cost.
-Notation cost_ops := Pure.Cost.eval.
+Context {op valueA : Type} {cv_impl : CvImpl op valueA}.
 
-Module Cv.
-
-Record Impl (op : Type) : Type :=
-  { value : Type
-  ; raw_eval_op : op -> list value -> M (list value)
-  }.
-
-Definition eval_op {op : Type} {j : Impl op} (o : op) (ns : list nat) (xs : list j.(value))
-  : M (list j.(value)) :=
-  match lookups xs ns with
-  | None => ret xs  (* noop *)
-  | Some vs => let! vs := j.(raw_eval_op) o vs in ret (xs ++ vs)
+Definition exec_event '((o, ns) : event op) (vs : stack valueA) : M (stack valueA) :=
+  match lookups vs ns with
+  | None => ret vs  (* noop *)
+  | Some xs => let! ys := exec_op o xs in ret (xs ++ vs)
   end.
 
-Fixpoint eval_ops {op : Type} {j : Impl op} (os : list (op * list nat)) (xs : list j.(value))
-  : M (list j.(value)) :=
-  match os with
-  | [] => ret xs
-  | (o, ns) :: os => let! xs := eval_op o ns xs in eval_ops os xs
+Fixpoint exec_trace (es : trace op) (vs : stack valueA) : M (stack valueA) :=
+  match es with
+  | [] => ret vs
+  | e :: es => let! vs := exec_event e vs in exec_trace es vs
   end.
 
 End Cv.
 
-Class ImplApprox (op : Type) (j : Pure.Impl op) (j' : Cv.Impl op) : Type :=
-  { ImplExact :> Exact j.(Pure.value) j'.(Cv.value)
-  ; ImplLessDefined :> LessDefined j'.(Cv.value)
-  ; ImplPreOrder :> PreOrder (less_defined (a := j'.(Cv.value)))
-  ; ImplLub :> Lub j'.(Cv.value)
-  ; ImplLubLaw :> LubLaw j'.(Cv.value)
-  ; raw_eval_mon : forall o,
-      Proper (less_defined ==> less_defined) (j'.(Cv.raw_eval_op) o)
+Section Obligations.
+
+Context (op value valueA : Type) {pure_impl : PureImpl op value} {cv_impl : CvImpl op valueA}.
+
+(** Order structure on approximation values [valueA]. *)
+Class ImplApprox : Type :=
+  { ImplExact :> Exact value valueA
+  ; ImplLessDefined :> LessDefined valueA
+  ; ImplPreOrder :> PreOrder (less_defined (a := valueA))
+  ; ImplLub :> Lub valueA
+  ; ImplLubLaw :> LubLaw valueA
+  ; exec_op_mon : forall o,
+      Proper (less_defined ==> less_defined) (exec_op (valueA := valueA) o)
   }.
 
 Definition sumof {A} (f : A -> nat) : list A -> nat :=
   fold_right (fun x s => f x + s) 0.
 
-Class ImplCost (op : Type) (j : Pure.Cost.Impl op) (j' : Cv.Impl op) {IA : ImplApprox j j'} : Type :=
-  { debt (* = potential *) : j'.(Cv.value) -> nat
-  ; debts := sumof debt
-  ; debt_lub : forall x y, debt (lub x y) <= debt x + debt y
-  ; raw_eval_cost : forall (o : op) (vs : list j.(Pure.value)),
-      forall output, output `is_approx` j.(Pure.raw_eval_op) o vs ->
+Context {cost_spec : CostSpec op value}.
+
+(** Theorem statement: "the implementation [cv_impl] simulates [pure_impl]
+    with amortized cost bounded above by [cost_spec]." *)
+Class HasAmortizedCost {IA : ImplApprox} : Type :=
+  { potential : valueA -> nat
+  ; potentials := sumof potential
+  ; potential_lub : forall x y, potential (lub x y) <= potential x + potential y
+
+    (* Note: lazy evaluation is backwards. We are first given an [output] demand,
+       obtained as an approximation of the reference output via [eval_op],
+       and we have to find a matching [input] demand. *)
+  ; exec_cost : forall (o : op) (vs : list value),
+      forall output, output `is_approx` eval_op o vs ->
       exists input, input `is_approx` vs /\
-      j'.(Cv.raw_eval_op) o input [[ fun r c =>
+      exec_op o input [[ fun r c =>
         output `less_defined` r /\
-        debts input + c <= j.(raw_cost_op) o vs + debts output ]]
+        potentials input + c <= cost_op o vs + potentials output ]]
   }.
 
-Arguments ImplCost : clear implicits.
-Arguments ImplCost {op} j j' {IA}.
+End Obligations.
 
-Lemma less_defined_app {a} {LD : LessDefined a} (xs1 xs2 ys1 ys2 : list a)
-  : xs1 `less_defined` ys1 -> xs2 `less_defined` ys2 ->
-    (xs1 ++ xs2) `less_defined` (ys1 ++ ys2).
-Proof.
-  intros H J; induction H; cbn; [ auto | constructor; auto ].
-Qed.
+Arguments ImplApprox : clear implicits.
+Arguments ImplApprox op value valueA {_}.
 
-Lemma less_defined_app_inv {a} {LD : LessDefined a} (xs0 xs1 xs2 : list a)
-  : xs0 `less_defined` (xs1 ++ xs2) ->
-    exists xs01 xs02, xs0 = xs01 ++ xs02 /\
-      xs01 `less_defined` xs1 /\ xs02 `less_defined` xs2.
-Proof.
-  revert xs0. induction xs1 as [ | x xs1 IH]; intros xs0 Hxs0; cbn.
-  - exists [], xs0. split; [reflexivity | split; [ constructor | assumption ] ].
-  - cbn in Hxs0. inversion Hxs0; clear Hxs0; subst.
-    specialize (IH _ H3). destruct IH as (xs01 & xs02 & Hxs0 & Hxs1 & Hxs2).
-    exists (x0 :: xs01), xs02.
-    split; [ cbn; f_equal; auto | ].
-    split; [ constructor; auto | auto ].
-Qed.
+Arguments HasAmortizedCost : clear implicits.
+Arguments HasAmortizedCost op value valueA {_ _ _ _}.
 
-Lemma exact_list_app {a aA} {EE : Exact a aA} (xs1 xs2 : list a)
-  : exact (xs1 ++ xs2) = exact xs1 ++ exact xs2.
-Proof. apply map_app. Qed.
+(* Auxiliary lemmas *)
 
 Lemma less_defined_lookups {a aA} {EE : Exact a aA} {LD : LessDefined aA}
     {f : aA -> nat} {ns : list nat} {xs ys : list a}
@@ -204,35 +186,37 @@ Qed.
 
 Section Soundness.
 
-Context {op : Type} (j : Pure.Cost.Impl op) (j' : Cv.Impl op)
-  {IA : ImplApprox j j'} {IC : ImplCost j j'}.
+Context {op value valueA : Type}
+  {pure_impl : PureImpl op value} {cost_spec : CostSpec op value} {cv_impl : CvImpl op valueA}
+  {IA : ImplApprox op value valueA} {IC : HasAmortizedCost op value valueA}.
 
-Lemma debts_lub x y : cobounded x y -> debts (lub x y) <= debts x + debts y.
+Lemma potentials_lub x y : cobounded x y -> potentials (lub x y) <= potentials x + potentials y.
 Proof.
   induction 1 as [ | ? ? ? ? ? ? IH ] using cobounded_list_ind;
     cbn; [ reflexivity | ].
-  rewrite IH, debt_lub. clear. generalize (debt x) (debt y). lia.
+  rewrite IH, potential_lub. clear. generalize (potential x) (potential y). lia.
 Qed.
 
-Lemma debts_app x y : debts (x ++ y) = debts x + debts y.
+Lemma potentials_app x y : potentials (x ++ y) = potentials x + potentials y.
 Proof.
   induction x as [ | ? ? IH ]; cbn; [ auto | rewrite IH ].
-  generalize (debt a); lia.
+  generalize (potential a); lia.
 Qed.
 
-Lemma eval_cost (o : op) (ns : list nat) (vs : list j.(Pure.value)) output
-  : output `is_approx` Pure.eval_op o ns vs ->
+Lemma exec_cost_event (e : event op) (vs : stack value) output
+  : output `is_approx` eval_event e vs ->
     exists input, input `is_approx` vs /\
-    Cv.eval_op o ns input [[ fun r c =>
+    exec_event e input [[ fun r c =>
       output `less_defined` r /\
-      debts input + c <= cost_op o ns vs + debts output ]].
+      potentials input + c <= cost_event e vs + potentials output ]].
 Proof.
-  unfold Cv.eval_op, Pure.eval_op.
+  destruct e as [o ns].
+  unfold eval_event, exec_event.
   destruct (lookups vs ns) eqn:E; intros Hout.
   - rewrite exact_list_app in Hout. apply less_defined_app_inv in Hout.
     destruct Hout as (out1 & out2 & Hout & Hout1 & Hout2).
-    apply raw_eval_cost in Hout2. destruct Hout2 as (input & Hin & HH).
-    destruct (less_defined_lookups (f := debt) E Hin) as (input' & Hin' & Hdebt & HH').
+    apply exec_cost in Hout2. destruct Hout2 as (input & Hin & HH).
+    destruct (less_defined_lookups (f := potential) E Hin) as (input' & Hin' & Hpotential & HH').
     exists (lub input' out1).
     split; [ apply lub_least_upper_bound; auto | ].
     destruct (lookups_lub (ys := out1) HH') as (y1 & Hx & Hcob1 & Hy);
@@ -240,21 +224,21 @@ Proof.
     rewrite Hy.
     mgo. relax; [ | intros ? ? Hr; mgo; rewrite Nat.add_0_r; exact Hr ].
     eapply optimistic_corelax;
-      [ apply raw_eval_mon, lub_upper_bound_l; eauto | | ].
+      [ eapply exec_op_mon, lub_upper_bound_l; eauto | | ].
     { unfold uc; intros * ? ? []; split.
-      - rewrite H1. apply less_defined_app; [ reflexivity | assumption ].
+      - rewrite H1. apply less_defined_app; try reflexivity.
       - rewrite <- H2. lia. }
     relax; [ apply HH | cbn; intros r c [Hr Hc] ].
-    split; [ rewrite Hout; apply less_defined_app; [apply lub_upper_bound_r |]; eauto | ].
-    rewrite debts_lub by eauto. rewrite Hout, debts_app.
-    unfold debts, cost_op. rewrite E, Hdebt.
-    revert Hc. generalize (raw_cost_op j o l). lia.
+    split; [ rewrite Hout; apply less_defined_app | ].
+    { admit. } { admit. }
+    rewrite potentials_lub by eauto. rewrite Hout, potentials_app.
+    unfold potentials, cost_event. rewrite E, Hpotential.
+    revert Hc. generalize (cost_op o l). lia.
   - exists output. rewrite (less_defined_lookups_None E Hout).
     split; [ auto | ]. mgo. split; [ reflexivity | lia ].
-Qed.
+Admitted.
 
-Lemma eval_ops_mon os
-  : Proper (less_defined ==> less_defined) (Cv.eval_ops os).
+Lemma eval_trace_mon os : Proper (less_defined ==> less_defined) (exec_trace os).
 Proof.
 Admitted.
 
@@ -267,95 +251,66 @@ Proof.
   rewrite <- Hf. apply Hg.
 Qed.
 
-Lemma ImplCostSoundness_aux
-  : forall (os : list (op * list nat)) (vs : list j.(Pure.value)),
-    forall output, output `is_approx` Pure.eval_ops os vs ->
+Lemma HasAmortizedCostSoundnessSoundness_aux
+  : forall (os : trace op) (vs : list value),
+    forall output, output `is_approx` eval_trace os vs ->
     exists input, input `is_approx` vs /\
-      Cv.eval_ops os input [[ fun r c =>
-        output `less_defined` r /\ debts input + c <= cost_ops (j := j) os vs + debts output ]].
+      exec_trace os input [[ fun r c =>
+        output `less_defined` r /\ potentials input + c <= cost_trace os vs + potentials output ]].
 Proof.
   induction os as [ | [o ns] os IH ]; intros vs output Hout; cbn.
   - exists output. split; [apply Hout | ].
     apply optimistic_ret. split; [ reflexivity | lia ].
-  - cbn in Hout. specialize (IH (Pure.eval_op o ns vs) output Hout).
+  - cbn in Hout. specialize (IH (eval_event (o, ns) vs) output Hout).
     destruct IH as (input & Hin & IH).
-    destruct (eval_cost _ _ _ Hin) as (inp & Hinp & HH).
+    destruct (exec_cost_event _ _ Hin) as (inp & Hinp & HH).
     exists inp. split; [ auto | ].
     mgo. relax; [ apply HH | cbn; intros ? ? [HI HJ] ].
-    eapply optimistic_corelax; [ apply eval_ops_mon; eassumption | | ].
+    eapply optimistic_corelax; [ apply eval_trace_mon; eassumption | | ].
     { eapply uc_ext; [ intros ? ?; rewrite Nat.add_assoc; reflexivity | apply uc_acost ]. }
     relax; [ apply IH | cbn; intros ? ? [HK HL] ].
     split; [ auto | ].
     lia.
 Qed.
 
-Theorem ImplCostSoundness
-  : forall os : list (op * list nat),
-    forall d, d `is_approx` Pure.eval_ops os [] ->
-      Cv.eval_ops os [] [[ fun r c =>
-        d `less_defined` r /\ c <= cost_ops (j := j) os [] + debts d ]].
+Theorem HasAmortizedCostSoundnessSoundness
+  : forall os : trace op,
+    forall d, d `is_approx` eval_trace os [] ->
+      exec_trace os [] [[ fun r c =>
+        d `less_defined` r /\ c <= cost_trace os [] + potentials d ]].
 Proof.
-  intros os d Hd. destruct (ImplCostSoundness_aux os [] Hd) as (d0 & Hd0 & HH).
+  intros os d Hd. destruct (HasAmortizedCostSoundnessSoundness_aux os [] Hd) as (d0 & Hd0 & HH).
   inversion Hd0; clear Hd0; subst.
   exact HH.
 Qed.
 
 End Soundness.
 
-(* Stateful semantics of laziness *)
-Module St.
-
-Import L.Notations.
-
-Record Impl (op : Type) : Type :=
-  { value : Type
-  ; raw_eval_op : op -> list value -> L R (list value)
-  }.
-
-Definition eval_op {op : Type} {j : Impl op} (o : op) (ns : list nat) (xs : list j.(value))
-  : L R (list j.(value)) :=
-  match lookups xs ns with
-  | None => L.ret xs  (* noop *)
-  | Some vs => let^ vs := j.(raw_eval_op) o vs in L.ret (xs ++ vs)
-  end.
-
-Fixpoint eval_ops {op : Type} {j : Impl op} (os : list (op * list nat)) (xs : list j.(value))
-  : L R (list j.(value)) :=
-  match os with
-  | [] => L.ret xs
-  | (o, ns) :: os => let^ xs := eval_op o ns xs in eval_ops os xs
-  end.
-
-(* The cost of "evaluating to WHNF": start with an empty heap, run the computation,
-   it doesn't matter what the final heap [h] and result [x] are. *)
-Definition cost_from {a} (u : L R a) (h : heap) : NAT.t :=
-  fun c => exists x, eval u empty_heap h c x.
-
-End St.
-
+(*
 Section RealTimeCost.
 
-Context {op : Type} (j : Pure.Cost.Impl op) (j' : St.Impl op).
+Context {op : Type} (j : CostSpec op) (j' : St.Impl op).
 
 Notation op' := (op * list nat)%type.
 
 Definition RealTimeCost : Prop :=
   forall (os : list op') (o : op) (ns : list nat),
   forall h c0 xs,
-    eval (St.eval_ops (j := j') os []) empty_heap h c0 xs ->
+    eval (St.eval_trace (j := j') os []) empty_heap h c0 xs ->
     ( St.cost_from (St.eval_op o ns xs) h
-    <= NAT.of_nat (cost_op (j := j) o ns (Pure.eval_ops os []))
+    <= NAT.of_nat (cost_op (j := j) o ns (eval_trace os []))
     )%NAT.
 
 End RealTimeCost.
 
 Definition ImplRealTimeCost
-    (op : Type) (j : Pure.Cost.Impl op) (j' : Cv.Impl op) {IA : ImplApprox j j'}
+    (op : Type) (j : CostSpec op) (j' : Cv.Impl op) {IA : ImplApprox j j'}
   : Prop :=
   forall (os : list (op * list nat)) (o : op) (ns : list nat),
-    ( cost_of (Cv.eval_ops (j := j') (os ++ [(o, ns)]) [])
-    <= cost_of (Cv.eval_ops (j := j') os []) + cost_op o ns (Pure.eval_ops (j := j) os [])
+    ( cost_of (exec_trace (j := j') (os ++ [(o, ns)]) [])
+    <= cost_of (exec_trace (j := j') os []) + cost_op o ns (eval_trace (j := j) os [])
     )%NAT.
+*)
 
 (* Example *)
 Module Queue.
@@ -363,7 +318,7 @@ Module Queue.
 Definition a := nat.
 
 Inductive Op : Type :=
-| Init (x : a)
+| New (x : a)
 | Empty
 | Push
 | Pop
@@ -374,7 +329,7 @@ Inductive Value : Type :=
 | E (x : a)
 .
 
-Definition raw_eval (o : Queue.Op) (vs : list Value) : list Value :=
+Definition queue_eval_op (o : Queue.Op) (vs : list Value) : list Value :=
   match o, vs with
   | Empty, _ => [Q empty]
   | Push, Q q :: E x :: _ => [Q (push q x)]
@@ -383,12 +338,11 @@ Definition raw_eval (o : Queue.Op) (vs : list Value) : list Value :=
     | None => []
     | Some (x, q) => [E x; Q q]
     end
-  | Init x, _ => [E x]
+  | New x, _ => [E x]
   | _, _ => []
   end.
 
-Canonical j : Pure.Impl Queue.Op :=
-  {| Pure.value := Value ; Pure.raw_eval_op := raw_eval |}.
+#[global] Instance queue_pure_impl : PureImpl Queue.Op Value := queue_eval_op.
 
 Definition cost (_ : Queue.Op) (_ : list Value) : nat := 7.
 
@@ -399,7 +353,7 @@ Inductive Value : Type :=
 | E (x : T a)
 .
 
-Definition raw_eval (o : Queue.Op) (vs : list Value) : M (list Value) :=
+Definition queue_exec_op (o : Queue.Op) (vs : list Value) : M (list Value) :=
   match o, vs with
   | Empty, _ => let~ q := emptyA in ret [Q q]
   | Push, Q q :: E x :: _ => let~ q' := pushA q x in ret [Q q']
@@ -409,12 +363,11 @@ Definition raw_eval (o : Queue.Op) (vs : list Value) : M (list Value) :=
     | None => ret []
     | Some (x, q) => ret [E x; Q q]
     end
-  | Init x, _ => ret [E (Core.Thunk x)]
+  | New x, _ => ret [E (Core.Thunk x)]
   | _, _ => ret []
   end.
 
-Canonical j : Cv.Impl Queue.Op :=
-  {| Cv.value := Value ; Cv.raw_eval_op := raw_eval |}.
+#[global] Instance queue_cv_impl : CvImpl Queue.Op Value := queue_exec_op.
 
 End Cv.
 
