src/Approx.v
@@ -33,6 +33,8 @@
 From Coq Require Import Arith List Lia Morphisms Relations.
 From Clairvoyance Require Import Core.
 
+Import ListNotations.
+
 Set Typeclasses Strict Resolution.
 
 Definition is_defined {a} (t : T a) : Prop :=
@@ -437,6 +439,31 @@ Proof.
       constructor; [ apply lub_upper_bound_r; eauto | ].
       apply IH; auto.
 Qed.
+
+Lemma less_defined_app {a} {LD : LessDefined a} (xs1 xs2 ys1 ys2 : list a)
+  : xs1 `less_defined` ys1 -> xs2 `less_defined` ys2 ->
+    (xs1 ++ xs2) `less_defined` (ys1 ++ ys2).
+Proof.
+  intros H J; induction H; cbn; [ auto | constructor; auto ].
+Qed.
+
+Lemma less_defined_app_inv {a} {LD : LessDefined a} (xs0 xs1 xs2 : list a)
+  : xs0 `less_defined` (xs1 ++ xs2) ->
+    exists xs01 xs02, xs0 = xs01 ++ xs02 /\
+      xs01 `less_defined` xs1 /\ xs02 `less_defined` xs2.
+Proof.
+  revert xs0. induction xs1 as [ | x xs1 IH]; intros xs0 Hxs0; cbn.
+  - exists [], xs0. split; [reflexivity | split; [ constructor | assumption ] ].
+  - cbn in Hxs0. inversion Hxs0; clear Hxs0; subst.
+    specialize (IH _ H3). destruct IH as (xs01 & xs02 & Hxs0 & Hxs1 & Hxs2).
+    exists (x0 :: xs01), xs02.
+    split; [ cbn; f_equal; auto | ].
+    split; [ constructor; auto | auto ].
+Qed.
+
+Lemma exact_list_app {a aA} {EE : Exact a aA} (xs1 xs2 : list a)
+  : exact (xs1 ++ xs2) = exact xs1 ++ exact xs2.
+Proof. apply map_app. Qed.
 
 Notation resp r1 r2 f f' := (forall x x', r1 x x' -> r2 (f x) (f' x')) (only parsing).
 
